backend/Allocproof_comp.v
@@ -2432,7 +2432,6 @@ Lemma MATCH_initial: forall v
           (fun b' : block => isGlobalBlock tge b' || getBlocks vals2 b') b = true ->
           DomT b = true) 
       (GFI: globalfunction_ptr_inject ge j)
-      (GDE: genvs_domain_eq ge tge)
       (HDomS: forall b : block, DomS b = true -> Mem.valid_block m1 b)
       (HDomT: forall b : block, DomT b = true -> Mem.valid_block m2 b),
 exists c2,
@@ -2507,7 +2506,7 @@ Proof. intros.
   intros CONTRA. solve[elimtype False; auto].
 
   destruct (core_initial_wd ge tge _ _ _ _ _ _ _  Inj
-     VInj J RCH PG GDE HDomS HDomT _ (eq_refl _))
+     VInj J RCH PG GDE_lemma HDomS HDomT _ (eq_refl _))
     as [AA [BB [CC [DD [EE [FF GG]]]]]].
   split.
     revert H1.
@@ -2597,7 +2596,6 @@ Proof.
 Qed.
 
 Lemma MATCH_afterExternal: forall
-      (GDE : genvs_domain_eq ge tge)
       mu st1 st2 m1 e vals1 m2 ef_sig vals2 e' ef_sig'
       (MemInjMu : Mem.inject (as_inj mu) m1 m2)
       (MatchMu: MATCH mu st1 m1 st2 m2)
@@ -4301,12 +4299,15 @@ Theorem transl_program_correct:
   (LTL_eff_sem hf) ge tge.
 Proof.
 intros.
-assert (GDE:= GDE_lemma).
  eapply simulations_lemmas.inj_simulation_plus_typed with
   (match_states:=fun x mu st m st' m' => MATCH mu st m st' m')
   (measure:=fun x => O).
 (*genvs_dom_eq*)
-  assumption.
+  apply GDE_lemma.
+(*ginfos_preserved*)
+ split; red; intros.
+   rewrite varinfo_preserved. apply gvar_info_refl.
+   rewrite symbols_preserved. trivial.
 (*match_wd*)
   intros; apply H.
 (*match_visible*)
