backend/RTLgenproof_comp.v
@@ -2869,7 +2869,6 @@ Lemma MATCH_initial: forall v
           (fun b' : block => isGlobalBlock tge b' || getBlocks vals2 b') b = true ->
           DomT b = true)
       (GFI: globalfunction_ptr_inject ge j)
-      (GDE: genvs_domain_eq ge tge)
       (HDomS: forall b : block, DomS b = true -> Mem.valid_block m1 b)
       (HDomT: forall b : block, DomT b = true -> Mem.valid_block m2 b),
 exists c2,
@@ -2938,7 +2937,7 @@ Proof. intros.
   intros CONTRA. solve[elimtype False; auto].
 
   destruct (core_initial_wd ge tge _ _ _ _ _ _ _  Inj
-     VInj J RCH PG GDE HDomS HDomT _ (eq_refl _))
+     VInj J RCH PG GDE_lemma HDomS HDomT _ (eq_refl _))
     as [AA [BB [CC [DD [EE [FF GG]]]]]].
   split.
     revert H1.
@@ -3021,7 +3020,6 @@ intuition.
 Qed.
 
 Lemma MATCH_afterExternal: forall
-      (GDE : genvs_domain_eq ge tge)
       mu st1 st2 m1 e vals1 m2 ef_sig vals2 e' ef_sig'
       (MemInjMu : Mem.inject (as_inj mu) m1 m2)
       (MatchMu: MATCH st1 mu st1 m1 st2 m2)
@@ -4760,12 +4758,14 @@ Theorem transl_program_correct:
   SM_simulation.SM_simulation_inject (cminsel_eff_sem hf)
    (rtl_eff_sem hf) ge tge.
 Proof.
-intros.
-assert (GDE:=GDE_lemma).
 apply simulations_lemmas.inj_simulation_star_wf with
   (match_states:=MATCH) (order :=lt_state).
 (*genvs_dom_eq*)
-  assumption.
+  apply GDE_lemma.
+(*ginfos_preserved*)
+ split; red; intros.
+   rewrite varinfo_preserved. apply gvar_info_refl.
+   rewrite symbols_preserved. trivial.
 (*MATCH_wd*)
   apply MATCH_wd. 
 (*MATCH_reachclosed*)
@@ -4794,7 +4794,7 @@ apply simulations_lemmas.inj_simulation_star_wf with
   { apply lt_state_wf. }
 (* after_external*)
   { intros.
-    specialize (MATCH_afterExternal GDE _ _ _ _ _ _ _ _ _ _ _ 
+    specialize (MATCH_afterExternal _ _ _ _ _ _ _ _ _ _ _ 
        MemInjMu MatchMu AtExtSrc AtExtTgt ValInjMu
        _ pubSrcHyp _ pubTgtHyp _ NuHyp _ _ _ _ _ INC GSep WDnu' SMvalNu'
        MemInjNu' RValInjNu' FwdSrc FwdTgt _ frgnSrcHyp _ frgnTgtHyp
