backend/Renumberproof_comp.v
@@ -409,7 +409,6 @@ exists st2' m2' U2 mu',
          Mem.perm m1 b1 (ofs - delta1) Max Nonempty)).
 Proof. intros.
   destruct MTCH as [MS [RC [PG [GFP [Glob [SMV [WD INJ]]]]]]].
-  assert (GDE:= GDE_lemma).
   assert (SymbPres := symbols_preserved).
 
   induction CS; intros; try (inv MS); try TR_AT. 
@@ -617,7 +616,7 @@ Proof. intros.
 { (* builtin *)
     rewrite restrict_sm_all, vis_restrict_sm, restrict_nest in AGREE; trivial. 
   inv H. 
-  exploit (inlineable_extern_inject ge tge); try eassumption.
+  exploit (inlineable_extern_inject _ _ GDE_lemma); try eassumption.
     eapply regset_get_list; eassumption.
   intros [mu' [v' [m'' [TEC [ResInj [MINJ' [UNMAPPED [LOOR [INC [SEP [GSEP [LOCALLOC [WD' [SMV' RC']]]]]]]]]]]]]]. 
  
@@ -793,7 +792,7 @@ split. (*?*)
 { (* nonobservable external function *) 
   rewrite  vis_restrict_sm, restrict_sm_all, restrict_nest in *; trivial.
   specialize (EFhelpers _ _ OBS); intros. 
-  exploit (inlineable_extern_inject ge tge); try eassumption.
+  exploit (inlineable_extern_inject _ _ GDE_lemma); try eassumption.
   intros [mu' [v' [m'' [TEC [ResInj [MINJ' [UNMAPPED
       [LOOR [INC [SEP [GSEP [LOCALLOC [WD' [SMV' RC']]]]]]]]]]]]]]. 
  
@@ -1005,7 +1004,6 @@ Proof. intros.
 Qed.
 
 Lemma MATCH_afterExternal: forall
-      (GDE : genvs_domain_eq ge tge)
       mu st1 st2 m1 e vals1 m2 ef_sig vals2 e' ef_sig'
       (MemInjMu : Mem.inject (as_inj mu) m1 m2)
       (MatchMu: MATCH mu st1 m1 st2 m2)
@@ -1250,7 +1248,6 @@ Lemma MATCH_initial: forall v
         (fun b' : Values.block => isGlobalBlock tge b' || getBlocks vals2 b') b =
          true -> DomT b = true)
   (GFI: globalfunction_ptr_inject ge j)
-  (GDE: genvs_domain_eq ge tge)
   (HDomS: forall b : Values.block, DomS b = true -> Mem.valid_block m1 b)
   (HDomT: forall b : Values.block, DomT b = true -> Mem.valid_block m2 b),
 exists c2,
@@ -1321,7 +1318,7 @@ Proof. intros.
   intros CONTRA. solve[elimtype False; auto].
 
   destruct (core_initial_wd ge tge _ _ _ _ _ _ _  Inj
-     VInj J RCH PG GDE HDomS HDomT _ (eq_refl _))
+     VInj J RCH PG GDE_lemma HDomS HDomT _ (eq_refl _))
     as [AA [BB [CC [DD [EE [FF GG]]]]]].
   split.
     eapply match_callstates; try eassumption.
@@ -1341,13 +1338,15 @@ Theorem transl_program_correct:
   SM_simulation.SM_simulation_inject 
     (rtl_eff_sem hf) (rtl_eff_sem hf) ge tge.
 Proof.
-intros.
-assert (GDE:= GDE_lemma).
  eapply simulations_lemmas.inj_simulation_plus with
   (match_states:=fun x mu st m st' m' => MATCH mu st m st' m')
   (measure:=fun x => O).
 (*genvs_dom_eq*)
-  assumption.
+  apply GDE_lemma.
+(*ginfos_preserved*)
+ split; red; intros.
+   rewrite varinfo_preserved. apply gvar_info_refl.
+   rewrite symbols_preserved. trivial.
 (*match_wd*)
   intros; apply H.
 (*match_visible*)
@@ -1375,7 +1374,7 @@ assert (GDE:= GDE_lemma).
 (*atExternal*)
   { apply MATCH_atExternal. } 
 (*afterExternal*)
-  { apply MATCH_afterExternal. assumption. }
+  { apply MATCH_afterExternal. }
 (*effcorediagram*)
 { intros. exploit MATCH_effcore_diagram; try eassumption.
   intros [st2' [m2' [U2 [mu' [CS' [INC [GSEP
