backend/Stackingproof_comp.v
@@ -4592,7 +4592,6 @@ Lemma MATCH_initial: forall v
         (fun b' : Values.block => isGlobalBlock tge b' || getBlocks vals2 b') b =
          true -> DomT b = true)
   (GFI: globalfunction_ptr_inject ge j)
-  (GDE: genvs_domain_eq ge tge)
   (HDomS: forall b : Values.block, DomS b = true -> Mem.valid_block m1 b)
   (HDomT: forall b : Values.block, DomT b = true -> Mem.valid_block m2 b),
 exists c2,
@@ -4671,7 +4670,7 @@ Proof. intros.
   intros CONTRA. solve[elimtype False; auto].
 
   destruct (core_initial_wd ge tge _ _ _ _ _ _ _  Inj
-     VInj J RCH PG GDE HDomS HDomT _ (eq_refl _))
+     VInj J RCH PG GDE_lemma HDomS HDomT _ (eq_refl _))
     as [AA [BB [CC [DD [EE [FF GG]]]]]]. simpl in *.  
 
   split. 2: rewrite initial_SM_as_inj; intuition.
@@ -4812,7 +4811,6 @@ Proof.
 Qed.
 
 Lemma MATCH_afterExternal: forall
-      (GDE : genvs_domain_eq ge tge)
       mu st1 st2 m1 e vals1 m2 ef_sig vals2 e' ef_sig'
       (MemInjMu : Mem.inject (as_inj mu) m1 m2)
       (MatchMu: MATCH st1 mu st1 m1 st2 m2)
@@ -6648,16 +6646,18 @@ Qed.
 
 (** The simulation proof *)
 Theorem transl_program_correct
-  (LNR: list_norepet (map fst (prog_defs prog))) :
+       (LNR: list_norepet (map fst (prog_defs prog))) :
   SM_simulation.SM_simulation_inject (Linear_eff_sem hf)
    (Mach_eff_sem hf return_address_offset) ge tge.
 Proof.
-intros.
-assert (GDE:= GDE_lemma). 
  eapply simulations_lemmas.inj_simulation_plus_typed with
   (match_states:=MATCH) (measure:=fun x => O).
 (*genvs_dom_eq*)
-  assumption.
+  apply GDE_lemma.
+(*ginfos_preserved*)
+ split; red; intros.
+   rewrite varinfo_preserved. apply gvar_info_refl.
+   rewrite symbols_preserved. trivial.
 (*MATCH_wd*)
   apply MATCH_wd. 
 (*MATCH_reachclosed*)
